\begin{problem}
Let p be the cubic polynomial that interpolates the function values
$f(0)$, $f(1)$, $f(2)$, and $f(3)$. Express $p(6)$ in terms of $f(0)$,
$f(1)$, $f(2)$, $f(3)$, and verify that your formula is correct when
$f$ is the function $ \{ f (x) = (x-3)^3 ; 0 \leq x \leq 6 \}$ What is the
uncertainty in the value of $p(6)$, if the uncertainty in each function
value is $\pm \epsilon$?
\end{problem}

%--------------------------------------------------------------------%

\begin{solution}  
We construct our polynomial using the Lagrange interpolation formula:
\begin{equation*}
p(x) = \sum_{i = 1}^n l_i(x)f(x_i)
\end{equation*}
obtaining the polynomial:
\begin{equation}
p(x) = \frac{(x-1)(x-2)(x-3)}{-6} f(0) + \frac{x(x-2)(x-3)}{2} f(1) + \frac{x(x-1)(x-3)}{-2} f(2) + \frac{x(x-1)(x-2)}{6} f(3)
\label{eq1t5}
\end{equation}
Then we get the formula for $p(6)$:
\begin{equation}
p(6) = -10f(0) + 36f(1) + - 45 f(2) + 20 f(3)
\label{eq2t5}
\end{equation}
Now if we use the function $f(x) = (x-3)^3$ we get that $f(0) = -27, f(1) = -8, f(2) = -1, f(3) = 0$. If we substitute these values in equation \ref{eq1t5} we get
\begin{equation*}
p(x) = -\frac{(x-1)(x-2)(x-3)}{-6} 27 - \frac{x(x-2)(x-3)}{2} 8 - \frac{x(x-1)(x-3)}{2}
\end{equation*}
which at $x = 6$ is 27, same as what the formula in equation \ref{eq2t5} gives when we substitute the functional values, therefore our formula is correct for that function.
\end{solution}

%%% Local Variables:
%%% TeX-master: "report.tex"
%%% End:
